WIP: Updated yesno_incr example to have global counter

fairness/examples/yesno_incr/yesno_incr.v
@@ -16,34 +16,21 @@ Import derived_laws_later.bi.
 Set Default Proof Using "Type".
 
 Definition yes_go : val :=
-  rec: "yes_go" "n" "b" :=
-    (if: CAS "b" #true #false
-      then "n" <- !"n" + #1
-       else #());;
-    "yes_go" "n" "b".
-
-Definition yes : val :=
-  λ: "b",
-    let: "n" := Alloc #0 in
-    yes_go "n" "b".
+  rec: "yes_go" "l" "n" :=
+    (if: CAS "l" "n" ("n"+#1)
+     then "yes_go" "l" ("n" + #2)
+     else "yes_go" "l" "n").
 
 Definition no_go : val :=
-  rec: "no_go" "n" "b" :=
-    (if: CAS "b" #false #true
-      then "n" <- !"n" + #1
-       else #());;
-    "no_go" "n" "b".
-
-Definition no : val :=
-  λ: "b",
-    let: "n" := Alloc #0 in
-    no_go "n" "b".
+  rec: "no_go" "l" "n" :=
+    (if: CAS "l" "n" ("n"+#1)
+     then "no_go" "l" ("n" + #2)
+     else "no_go" "l" "n").
 
 Definition start : val :=
-  λ: <>,
-    let: "b" := Alloc #true in
-    (Fork (yes "b") ;;
-    Fork (no "b")).
+  λ: "l",
+    (Fork (yes_go "l" #0) ;;
+    Fork (no_go "l" #1)).
 
 (** * Definition of the model! *)
 
@@ -64,12 +51,11 @@ Qed.
 #[global] Instance YN_inhabited: Inhabited YN.
 Proof. exact (populate Y). Qed.
 
-
-Inductive yntrans: nat*bool -> option YN -> nat*bool -> Prop :=
-| yes_trans n : yntrans (n, true) (Some Y) (n, false) (* < *)
-| yes_fail n : yntrans (n, false) (Some Y) (n, false) (* ≤ *)
-| no_trans n : yntrans (n, false) (Some No) (S n, true) (* < *)
-| no_fail n : yntrans (n, true) (Some No) (n, true) (* ≤ *)
+Inductive yntrans: nat -> option YN -> nat -> Prop :=
+| yes_trans n : Nat.even n → yntrans n (Some Y) (S n)
+| yes_fail n : Nat.odd n → yntrans n (Some Y) n
+| no_trans n : Nat.odd n → yntrans n (Some No) (S n)
+| no_fail n : Nat.even n → yntrans n (Some No) n
 .
 
 Definition yn_live_roles : gset YN := {[ No; Y ]}.
@@ -77,14 +63,14 @@ Definition yn_live_roles : gset YN := {[ No; Y ]}.
 Lemma live_spec_holds :
   forall s ρ s', yntrans s (Some ρ) s' -> ρ ∈ yn_live_roles.
 Proof.
-  intros [n b] yn [n' ?] Htrans. rewrite /yn_live_roles.
+  intros n yn n' Htrans. rewrite /yn_live_roles.
   inversion Htrans; simplify_eq; try set_solver; try lia; destruct n'; try set_solver; lia.
 Qed.
 
 Definition the_fair_model: FairModel.
 Proof.
   refine({|
-            fmstate := nat * bool;
+            fmstate := nat;
             fmrole := YN;
             fmtrans := yntrans;
             live_roles _ := yn_live_roles;
@@ -156,298 +142,195 @@ Section proof.
     rewrite -!own_op. iApply own_update. apply excl_auth_update.
   Qed.
 
-  Definition yesno_inv_inner b :=
-    (∃ N B,
+  Definition yesno_inv_inner n :=
+    (∃ N,
           frag_free_roles_are ∅ ∗
-          frag_model_is (N, B) ∗ b ↦ #B ∗
-          (if B
-           then auth_yes_at N ∗ auth_no_at N
-           else auth_yes_at (N+1) ∗ auth_no_at N)
-    )%I.
-  Definition yesno_inv b := inv Ns (yesno_inv_inner b).
+          frag_model_is N ∗ n ↦ #N ∗
+          (if (Nat.even N)
+           then auth_yes_at N ∗ auth_no_at (N+1)
+           else auth_yes_at (N+1) ∗ auth_no_at N))%I.
+  Definition yesno_inv n := inv Ns (yesno_inv_inner n).
 
-  Lemma yes_go_spec tid n b (N: nat) f (Hf: f > 40):
-    {{{ yesno_inv b ∗ has_fuel tid Y f ∗ n ↦ #N ∗ yes_at N }}}
-      yes_go #n #b @ tid
+  Lemma yes_go_spec tid n (N: nat) f (Hf: f > 40):
+    {{{ yesno_inv n ∗ has_fuel tid Y f ∗ yes_at N }}}
+      yes_go #n #N @ tid
     {{{ RET #(); tid ↦M ∅ }}}.
   Proof.
     iLöb as "Hg" forall (N f Hf).
-
-    iIntros (Φ) "(#Hinv & Hf & HnN & Hyes) Hk".
+    iIntros (Φ) "(#Hinv & Hf & Hyes) Hk".
     wp_lam.
     wp_pures.
     wp_bind (CmpXchg _ _ _).
-    assert (∀ s, Atomic s (CmpXchg #b #true #false)) by apply _.
     iApply wp_atomic.
-    iInv Ns as (M B) "(>HFR & >Hmod & >Bb & Hauths)" "Hclose".
-    destruct B; iDestruct "Hauths" as "[>Hay >Han]".
+    iInv Ns as (M) "(>HFR & >Hmod & >Hn & Hauths)" "Hclose".
+    destruct (Nat.even M) eqn:Heqn; iDestruct "Hauths" as "[>Hay >Han]".
     - iDestruct (yes_agree with "Hyes Hay") as "%Heq".
-
-      (* TODO *)
       rewrite -has_fuel_fuels.
       iApply (wp_cmpxchg_suc_step_singlerole _ tid (Y: fmrole the_fair_model) _ 55%nat _
-                                             (M, true) (M, false)
+                                             M (M + 1)
              with "[$]"); eauto.
-
+      { by do 3 f_equiv. }
       { simpl. lia. }
-      { econstructor. }
+      { rewrite Nat.add_1_r. econstructor. eauto. }
       iModIntro.
       iIntros "!> (Hb & Hmod & HFR & Hf)".
-      iMod (yes_update (M+1) with "[$]") as "[Hay Hyes]".
+      iMod (yes_update (M + 2) with "[$]") as "[Hay Hyes]".
       iMod ("Hclose" with "[Hmod Hay Han Hb HFR]").
-      { iNext. iExists _, _. iFrame. }
+      { iNext. iExists _. iFrame. rewrite Nat2Z.inj_add.
+        subst. iFrame.
+        rewrite Nat.add_1_r.
+        rewrite Nat.even_succ.
+        rewrite -Nat.negb_even. rewrite Heqn. simpl. iFrame.
+        rewrite Nat.add_1_r.
+        replace (S (S N)) with (N + 2) by lia. iFrame. }
       iModIntro. rewrite decide_True; last first.
       { set_solver. }
-
-
       rewrite has_fuel_fuels.
       wp_pures.
-      wp_load.
-      wp_pures.
-      wp_store.
-      wp_pures.
-
-      simplify_eq.
-
-      rewrite -has_fuel_fuels.
-      iApply ("Hg" with "[] [Hyes HnN Hf] [$]"); last first.
-      { iFrame "∗#". by rewrite Nat2Z.inj_add. }
+      replace (Z.of_nat N + 2)%Z with (Z.of_nat (N + 2)) by lia.
+      iApply ("Hg" with "[] [Hyes Hf] [$]"); last first.
+      { iFrame "∗#". rewrite has_fuel_fuels.
+        subst. iFrame. }
       iPureIntro; lia.
     - iDestruct (yes_agree with "Hyes Hay") as "%Heq". rewrite -> Heq in *.
-
       rewrite -has_fuel_fuels.
       iApply (wp_cmpxchg_fail_step_singlerole _ tid (Y: fmrole the_fair_model) _ 50%nat _
-                                             (M, false) (M, false)
+                                             M M
              with "[$]"); eauto.
+      { intros Hne. simplify_eq. lia. }
       { simpl. lia. }
-      { econstructor. }
-
+      { econstructor. rewrite -Nat.negb_even. rewrite Heqn. done. }
       iIntros "!>!> (Hb & Hmod & HFR & Hf)".
-      (* iMod (yes_update (N-1) with "[$]") as "[Hay Hyes]". *)
       iMod ("Hclose" with "[Hmod Hb Hay Han HFR]").
-      { iNext. simplify_eq. iExists _, _. iFrame. iFrame. }
-
+      { iNext. simplify_eq. iExists _. iFrame.
+        subst. iFrame.
+        rewrite Nat.add_1_r. rewrite Heqn. iFrame. }
       rewrite decide_True; last first.
       { set_solver. }
-
       iModIntro.
       wp_pures.
       rewrite -has_fuel_fuels.
-      iApply ("Hg" with "[] [Hyes HnN Hf] [$]"); last first.
+      iApply ("Hg" with "[] [Hyes Hf] [$]"); last first.
       { iFrame "∗#". }
       iPureIntro; lia.
   Qed.
 
-  Lemma yes_spec tid b f (Hf: f > 50):
-    {{{ yesno_inv b ∗ has_fuel tid Y f ∗ yes_at 0 }}}
-      yes #b @ tid
-    {{{ RET #(); tid ↦M ∅ }}}.
-  Proof.
-    iIntros (Φ) "(#Hinv & Hf & Hyes) Hk".
-
-    wp_lam.
-    wp_pures.
-    wp_bind (Alloc _).
-
-    rewrite has_fuels_gt_1; last by solve_fuel_positive.
-
-    iApply (wp_alloc_nostep _ _ _ _ {[Y := _]}%nat with "[Hf]").
-    { apply map_non_empty_singleton. }
-    { rewrite fmap_insert fmap_empty. done. }
-    iNext. iIntros (n) "(HnN & _ & Hf)".
-    rewrite -has_fuel_fuels.
-
-    wp_pures.
-
-    rewrite -has_fuel_fuels.
-
-    iApply (yes_go_spec with "[-Hk]"); try iFrame.
-    { lia. }
-    { iFrame "#∗". }
-  Qed.
-
-  Lemma no_go_spec tid n b (N: nat) f (Hf: f > 40):
-    {{{ yesno_inv b ∗ has_fuel tid No f ∗ n ↦ #N ∗ no_at N }}}
-      no_go #n #b @ tid
+  Lemma no_go_spec tid n (N: nat) f (Hf: f > 40):
+    {{{ yesno_inv n ∗ has_fuel tid No f ∗ no_at N }}}
+      no_go #n #N @ tid
     {{{ RET #(); tid ↦M ∅ }}}.
   Proof.
     iLöb as "Hg" forall (N f Hf).
-
-    iIntros (Φ) "(#Hinv & Hf & HnN & Hno) Hk".
-
+    iIntros (Φ) "(#Hinv & Hf & Hno) Hk".
     wp_lam.
     wp_pures.
     wp_bind (CmpXchg _ _ _).
-
-    assert (∀ s, Atomic s (CmpXchg #b #true #false)) by apply _.
-
     iApply wp_atomic.
-
-    iInv Ns as (M B) "(>HFR & >Hmod & >Bb & Hauths)" "Hclose".
-    destruct B; iDestruct "Hauths" as "[>Hay >Han]"; last first.
+    iInv Ns as (M) "(>HFR & >Hmod & >Hn & Hauths)" "Hclose".
+    destruct (Nat.even M) eqn:Heqn; iDestruct "Hauths" as "[>Hay >Han]"; last first.
     - iDestruct (no_agree with "Hno Han") as "%Heq".
-
-      (* TODO *)
       rewrite -has_fuel_fuels.
-
       iApply (wp_cmpxchg_suc_step_singlerole _ tid (No: fmrole the_fair_model) _ 55%nat _
-                                             (M, false) (S M, true)
+                                             M (S M)
                with "[$]"); eauto.
+      { by do 3 f_equiv. }
       { simpl. lia. }
-      { econstructor. }
+      { econstructor. rewrite -Nat.negb_even. rewrite Heqn. done. }
       iModIntro.
       iIntros "!> (Hb & Hmod & HFR & Hf)".
-      iMod (no_update (S M) with "[$]") as "[Han Hno]".
+      iMod (no_update (M + 2) with "[$]") as "[Han Hno]".
       iMod ("Hclose" with "[Hmod Hay Han Hb HFR]").
-      { iNext. iExists _, _. iFrame.
-        iApply (own_proper with "Hay"). f_equiv. apply leibniz_equiv_iff. lia. }
-
+      { iNext. iExists _. iFrame. subst.
+        rewrite Nat.add_1_r.
+        rewrite Nat.even_succ.
+        rewrite -Nat.negb_even. rewrite Heqn. simpl. iFrame.
+        rewrite Nat.add_1_r.
+        replace (S (S N)) with (N + 2) by lia.
+        iFrame.
+        iEval (rewrite -Nat.add_1_r).
+        rewrite Nat2Z.inj_add.
+        iFrame. }
       iModIntro. rewrite decide_True; last first.
       { set_solver. }
-
       rewrite has_fuel_fuels.
       wp_pures.
-      wp_load.
-      wp_pures.
-      wp_store.
-      wp_pures.
-
       rewrite -has_fuel_fuels.
-      iApply ("Hg" with "[] [Hno HnN Hf] [$]"); last first.
-      { iFrame "∗#". simplify_eq. iEval (rewrite -Nat.add_1_r).
-        by rewrite Nat2Z.inj_add. }
+      replace (Z.of_nat N + 2)%Z with (Z.of_nat (N + 2)) by lia.
+      iApply ("Hg" with "[] [Hno Hf] [$]"); last first.
+      { iFrame "∗#". simplify_eq. done. }
       iPureIntro; lia.
     - iDestruct (no_agree with "Hno Han") as "%Heq". rewrite -> Heq in *.
-
-      rewrite -has_fuel_fuels. assert (M = N) by lia. simplify_eq.
+      rewrite -has_fuel_fuels. simplify_eq.
       iApply (wp_cmpxchg_fail_step_singlerole _ tid (No: fmrole the_fair_model) _ 50%nat _
-                                             (N, true) (N, true)
+                                             M M
              with "[$]"); eauto.
+      { intros Hneq. simplify_eq. lia. }
       { simpl. lia. }
-      { econstructor. }
+      { econstructor. eauto. }
       iIntros "!>!> (Hb & Hmod & HFR & Hf)".
       iMod ("Hclose" with "[Hmod Hb Hay Han HFR]").
-      { iNext. simplify_eq. iExists _, _. iFrame. iFrame. }
-
+      { iNext. simplify_eq. iExists _. iFrame.
+        rewrite Heqn. iFrame. }
       rewrite decide_True; last first.
       { set_solver. }
-
       iModIntro.
       wp_pures.
-
       rewrite -has_fuel_fuels.
-      iApply ("Hg" with "[] [Hno HnN Hf] [$]"); last first.
+      iApply ("Hg" with "[] [Hno Hf] [$]"); last first.
       { iFrame "∗#". }
       iPureIntro; lia.
-  Qed.
-
-  Lemma no_spec tid b f (Hf: f > 50):
-    {{{ yesno_inv b ∗ has_fuel tid No f ∗ no_at 0 }}}
-      no #b @ tid
-    {{{ RET #(); tid ↦M ∅ }}}.
-  Proof.
-    iIntros (Φ) "(#Hinv & Hf & Hyes) Hk".
-
-    wp_lam.
-    wp_pures.
-    wp_bind (Alloc _).
-
-    rewrite has_fuels_gt_1; last by solve_fuel_positive.
-
-    iApply (wp_alloc_nostep _ _ _ _ {[No := _]}%nat with "[Hf]").
-    { apply map_non_empty_singleton. }
-    { rewrite fmap_insert fmap_empty. done. }
-    iNext. iIntros (n) "(HnN & _ & Hf)".
-    rewrite -has_fuel_fuels.
-
-    wp_pures.
-
-    rewrite -has_fuel_fuels.
-
-    iApply (no_go_spec with "[-Hk]"); try iFrame.
-    { lia. }
-    { iFrame "Hinv". done. }
   Qed.
 
 End proof.
 
-
 Section proof_start.
-  Context `{!heapGS Σ the_model, !yesnoPreG Σ}.
+  Context `{!heapGS Σ the_model, !yesnoG Σ}.
   Let Ns := nroot .@ "yes_no".
 
-  Lemma start_spec tid f (Hf: f > 60):
-    {{{ frag_model_is (0, true) ∗ frag_free_roles_are ∅ ∗
-        has_fuels tid {[ Y := f; No := f ]} }}}
-      start #() @ tid
+  Lemma start_spec tid n f (Hf: f > 60):
+    {{{ yesno_inv n ∗ has_fuels tid {[ Y := f; No := f ]} ∗ yes_at 0 ∗ no_at 1 }}}
+      start #n @ tid
     {{{ RET #(); tid ↦M ∅ }}}.
   Proof using All.
-    iIntros (Φ) "[Hst [HFR Hf]] Hkont". unfold start.
-
+    iIntros (Φ) "(#Hinv & Hf & Hyes_at & Hno_at) HΦ". unfold start.
     wp_pures.
-
-    wp_bind (Alloc _).
-    iApply (wp_alloc_nostep _ _ _ _ {[Y := _; No := _]} with "[Hf]").
-    { apply insert_non_empty. }
-    { rewrite has_fuels_gt_1; last solve_fuel_positive.
-      rewrite !fmap_insert fmap_empty //. }
-
-    iIntros "!>" (l) "(Hl & _ & Hf)".
-
-    wp_pures.
-
-    (* Allocate the invariant. *)
-    iMod (own_alloc (●E 0  ⋅ ◯E 0))%nat as (γ_yes_at) "[Hyes_at_auth Hyes_at]".
-    { apply auth_both_valid_2; eauto. by compute. }
-    iMod (own_alloc (●E 0  ⋅ ◯E 0))%nat as (γ_no_at) "[Hno_at_auth Hno_at]".
-    { apply auth_both_valid_2; eauto. by compute. }
-
-    pose (the_names := {|
-     yes_name := γ_yes_at;
-     no_name := γ_no_at;
-    |}).
-
-    iApply fupd_wp.
-    iMod (inv_alloc Ns _ (yesno_inv_inner l) with "[-Hkont Hf Hyes_at Hno_at]") as "#Hinv".
-    { iNext. unfold yesno_inv_inner. iExists 0, true. by iFrame. }
-    iModIntro.
-
     wp_bind (Fork _).
     rewrite has_fuels_gt_1; last solve_fuel_positive.
     iApply (wp_fork_nostep _ tid _ _ _ {[ No ]} {[ Y ]} {[Y := _; No := _]}
              with "[Hyes_at] [- Hf] [Hf]");
       [ set_solver | by apply insert_non_empty |  | | | rewrite !fmap_insert fmap_empty // ];
       [set_solver | |].
-    { iIntros (tid') "!> Hf". iApply (yes_spec with "[-]"); last first.
+    { iIntros (tid') "!> Hf".
+      replace 0%Z with (Z.of_nat 0) by lia.
+      iApply (yes_go_spec with "[-]"); last first.
       + by eauto.
       + rewrite map_filter_insert_True; last set_solver.
         rewrite map_filter_insert_not; last set_solver.
         rewrite map_filter_empty insert_empty.
         rewrite has_fuel_fuels. by iFrame "#∗".
       + lia. }
-
     iIntros "!> Hf".
     rewrite map_filter_insert_not; last set_solver.
     rewrite map_filter_insert_True; last set_solver.
     rewrite map_filter_empty insert_empty.
-
     iModIntro.
     wp_pures.
-
     rewrite has_fuels_gt_1; last solve_fuel_positive.
-    iApply (wp_fork_nostep _ tid _ _ _ ∅ {[ No ]} {[No := _]} with "[Hno_at] [Hkont] [Hf]");
+    iApply (wp_fork_nostep _ tid _ _ _ ∅ {[ No ]} {[No := _]} with "[Hno_at] [HΦ] [Hf]");
       [ set_solver | by apply insert_non_empty |  | | | rewrite !fmap_insert fmap_empty // ];
       [set_solver | |].
-    { iIntros (tid') "!> Hf". iApply (no_spec with "[-]"); last first.
+    { iIntros (tid') "!> Hf".
+      replace 1%Z with (Z.of_nat 1) by lia.
+      iApply (no_go_spec with "[-]"); last first.
       + by eauto.
       + rewrite map_filter_insert_True; last set_solver.
         rewrite map_filter_empty insert_empty.
         rewrite has_fuel_fuels. by iFrame "#∗".
       + lia. }
-
     iNext. iIntros "[Hf _]".
-    iApply "Hkont". iModIntro. iApply (equiv_wand with "Hf"). do 2 f_equiv.
+    iApply "HΦ". iModIntro. iApply (equiv_wand with "Hf"). do 2 f_equiv.
     rewrite dom_empty_iff_L map_filter_empty_iff.
     intros ???. set_solver.
   Qed.
+
 End proof_start.
